%
% Copyright © 2016 Peeter Joot.  All Rights Reserved.
% Licenced as described in the file LICENSE under the root directory of this GIT repository.
%
%{
\input{../blogpost.tex}
\renewcommand{\basename}{gradientGreensFunction}
\renewcommand{\dirname}{notes/phy1520/}
%\newcommand{\dateintitle}{}
%\newcommand{\keywords}{}

\input{../peeter_prologue_print2.tex}

\usepackage{peeters_layout_exercise}
\usepackage{peeters_braket}
\usepackage{peeters_figures}
\usepackage{siunitx}

\beginArtNoToc

\generatetitle{Green's function for gradient in Euclidean spaces}
%\chapter{Green's function for gradient in Euclidean spaces}
%\label{chap:gradientGreensFunction}

In \citep{doran2003gap} it is stated that the Green's function for the gradient is

\begin{dmath}\label{eqn:gradientGreensFunction:20}
   G(x, x') = \inv{S_n} \frac{x - x'}{\Abs{x-x'}^n},
\end{dmath}

where \( n \) is the dimension of the space, \( S_n \) is the area of the unit sphere, and 
\begin{equation}\label{eqn:gradientGreensFunction:40}
   \grad G = \grad \cdot G = \delta(x - x').
\end{equation}

What I'd like to do here is verify that this Green's function operates as asserted.  
Note that I am following the convention of the text, where vectors are generally written without boldface unless attention is restricted to \R{3}.

Let's start with checking that the gradient of the Green's function is zero everywhere that \( x \ne x' \)

\begin{dmath}\label{eqn:gradientGreensFunction:100}
\spacegrad \inv{\Abs{x - x'}^n} 
=
-\frac{n}{2} \frac{e^\nu \partial_\nu (x_\mu - x_\mu')(x^\mu - {x^\mu}')}{\Abs{x - x'}^{n+2}}
=
-\frac{n}{2} 2 \frac{e^\nu (x_\mu - x_\mu') \delta_\nu^\mu }{\Abs{x - x'}^{n+2}}
=
-n \frac{ x - x'}{\Abs{x - x'}^{n+2}}.
\end{dmath}

This means that we have, everywhere that \( x \ne x' \)

\begin{dmath}\label{eqn:gradientGreensFunction:120}
\spacegrad \cdot G
=
\inv{S_n} \lr{ \frac{\spacegrad \cdot \lr{x - x'}}{\Abs{x - x'}^{n}} + \lr{ \spacegrad \inv{\Abs{x - x'}^{n}} } \cdot \lr{ x - x'} }
=
\inv{S_n} \lr{ \frac{n}{\Abs{x - x'}^{n}} + \lr{ -n \frac{x - x'}{\Abs{x - x'}^{n+2} } \cdot \lr{ x - x'} } }
= 0.
\end{dmath}

Next, consider the curl of the Green's function.  
Zero curl will mean that we have \( \grad G = \grad \cdot G = G \lgrad \).

\begin{dmath}\label{eqn:gradientGreensFunction:140}
S_n (\grad \wedge G)
=
\frac{\grad \wedge (x-x')}{\Abs{x - x'}^{n}}
+
\grad \inv{\Abs{x - x'}^{n}} \wedge (x-x')
=
\frac{\grad \wedge (x-x')}{\Abs{x - x'}^{n}}
- \cancel{n
\frac{x - x'}{\Abs{x - x'}^{n}} \wedge (x-x')}.
\end{dmath}

However, 

\begin{dmath}\label{eqn:gradientGreensFunction:160}
\grad \wedge (x-x')
=
\grad \wedge x
=
e^\mu \wedge e_\nu \partial_\mu x^\nu
=
e^\mu \wedge e_\nu \delta_\mu^\nu
=
e^\mu \wedge e_\mu.
\end{dmath}

For any metric where \( e_\mu \propto e^\mu \), which is the case in all the ones with physical interest (i.e. \R{3} and Minkowski space), \( \grad \wedge G \) is zero.

Having shown that the gradient of the (presumed) Green's function is zero everwhere that \( x \ne x' \), the guts of the 
demonstration can now proceed.  We wish to evaluate the gradient weighted convolution of the Green's function using the Fundamental Theorem of (Geometric) Calculus.  Here the gradient acts bidirectionally on both the gradient and the test function.  Working in primed coordinates so that the final result is in terms of the unprimed, we have

\begin{dmath}\label{eqn:gradientGreensFunction:60}
   \int_V G(x,x') d^n x' \lrgrad' F(x') 
   = \int_{\partial V} G(x,x') d^{n-1} x' F(x').
\end{dmath}

Let \( d^n x' = dV' I \), \( d^{n-1} x' n = dA' I \), where \( n = n(x') \) is the outward normal to the area element \( d^{n-1} x' \).
From this point on, lets restrict attention to Euclidean spaces, where \( n^2 = 1 \).  In that case

\begin{dmath}\label{eqn:gradientGreensFunction:80}
\int_V dV' G(x,x') \lrgrad' F(x') 
=
\int_V dV' \lr{G(x,x') \lgrad'} F(x') 
+
\int_V dV' G(x,x') \lr{ \rgrad' F(x') }
= \int_{\partial V} dA' G(x,x') n F(x').
\end{dmath}

Here, the pseudoscalar \( I \) has been factored out by commuting it with \( G \), using \( G I = (-1)^{n-1} I G \), and then pre-multiplication with \( 1/((-1)^{n-1} I ) \).  

Each of these integrals can be considered in sequence.  A convergence bound is required of the multivector test function \( F(x' \) on the infinite surface \( \partial V \).  Since it's true that

\begin{dmath}\label{eqn:gradientGreensFunction:180}
\Abs{ \int_{\partial V} dA' G(x,x') n F(x') }
\ge
\int_{\partial V} dA' \Abs{ G(x,x') n F(x') },
\end{dmath}

then it is sufficient to require that 

\begin{dmath}\label{eqn:gradientGreensFunction:200}
\lim_{x' \rightarrow \infty} \Abs{ \frac{x -x'}{\Abs{x - x'}^n} n(x') F(x') } \rightarrow 0,
\end{dmath}

in order to kill off the surface integral.  Evaluating the integral on a hypersphere centered on \( x \) where \( x - x' = n \Abs{x - x'} \), that is

\begin{dmath}\label{eqn:gradientGreensFunction:260}
\lim_{x' \rightarrow \infty} \frac{ \Abs{F(x')}}{\Abs{x - x'}^{n-1}} \rightarrow 0.
\end{dmath}

Given such a constraint, that leaves

\begin{dmath}\label{eqn:gradientGreensFunction:220}
\int_V dV' \lr{G(x,x') \lgrad'} F(x') 
=
-\int_V dV' G(x,x') \lr{ \rgrad' F(x') }.
\end{dmath}

The LHS is zero everywhere that \( x \ne x' \) so it can be restricted to a spherical ball around \( x \), which allows the test function \( F \) to be pulled out of the integral

\begin{dmath}\label{eqn:gradientGreensFunction:240}
\int_V dV' \lr{G(x,x') \lgrad'} F(x') 
=
\lim_{\epsilon \rightarrow 0}
\int_{\Abs{x - x'} < \epsilon} dV' \lr{G(x,x') \lgrad'} F(x') 
=
\lr{ \lim_{\epsilon \rightarrow 0}
I^{-1} \int_{\Abs{x - x'} < \epsilon} I dV' \lr{G(x,x') \lgrad'} 
} F(x) 
=
\lr{ \lim_{\epsilon \rightarrow 0}
(-1)^{n-1} I^{-1} \int_{\Abs{x - x'} < \epsilon} G(x,x') d^n x' \lgrad'
} F(x) 
=
\lr{ \lim_{\epsilon \rightarrow 0}
(-1)^{n-1} I^{-1} \int_{\Abs{x - x'} = \epsilon} G(x,x') d^{n-1} x'
} F(x)
=
\lr{ \lim_{\epsilon \rightarrow 0}
(-1)^{n-1} I^{-1} \int_{\Abs{x - x'} = \epsilon} G(x,x') dA' I n
} F(x)
=
\lr{ \lim_{\epsilon \rightarrow 0}
\int_{\Abs{x - x'} = \epsilon} dA' G(x,x') n
} F(x)
=
\lr{ \lim_{\epsilon \rightarrow 0}
\int_{\Abs{x - x'} = \epsilon} dA' \frac{\epsilon n}{S_n \epsilon^n} n
} F(x)
=
\lim_{\epsilon \rightarrow 0}
\frac{F(x)}{S_n \epsilon^{n-1}}
\int_{\Abs{x - x'} = \epsilon} dA'
=
\lim_{\epsilon \rightarrow 0}
\frac{F(x)}{S_n \epsilon^{n-1}}
S_n \epsilon^{n-1}.
= 
F(x).
\end{dmath}

So, provided the test function is constrained by \cref{eqn:gradientGreensFunction:260}, we have

\begin{dmath}\label{eqn:gradientGreensFunction:280}
F(x) = -\int_V dV' G(x,x') \lr{ \grad' F(x') }.
\end{dmath}

In particular, should we have a first order gradient equation

\begin{dmath}\label{eqn:gradientGreensFunction:300}
\spacegrad' F(x') = M(x'),
\end{dmath}

the inverse of this equation is given by
\begin{dmath}\label{eqn:gradientGreensFunction:320}
F(x) = -\int_V dV' G(x,x') M(x').
\end{dmath}

There is a slightly annoying negative sign in this convoluation integral, which is important to keep in mind.  If desired, it can be eliminated by a variable substitution

\begin{dmath}\label{eqn:gradientGreensFunction:340}
F(y) 
= -\int_V dV' G(y,x') M(x')
= -\int_V dV G(y,x) M(x),
\end{dmath}

or
%\begin{dmath}\label{eqn:gradientGreensFunction:360}
\boxedEquation{eqn:gradientGreensFunction:360}{
F(y) 
= \int_V dV G(x, y) M(x).
}
%\end{dmath}

% \paragraph{Future thought}
% FIXME: how to generalize to mixed signature spaces.
%since I don't know what it means to calculate the surface area of a unit sphere in a mixed signature space.

%}
\EndArticle
