%
% Copyright © 2012 Peeter Joot.  All Rights Reserved.
% Licenced as described in the file LICENSE under the root directory of this GIT repository.
%

\label{chap:hermiteDerivativeRecurranceRelation}

%\blogpage{http://sites.google.com/site/peeterjoot2/math2012/hermiteDerivativeRecurranceRelation.pdf}
%\date{Jan 3, 2012}

For a QM problem I had need of a recurrence relation for Hermite polynomials.  I found it in \citep{abramowitz1964handbook}, but thought I had try to derive the relation myself.

The starting point I will use is the Rodgigues' formula definition of the Hermite polynomials

\begin{equation}\label{eqn:hermiteDerivativeRecurranceRelation:10}
H_n = (-1)^n e^{x^2} \frac{d^n}{dx^n} e^{-x^2}
\end{equation}

Let us write \(D = d/dx\), and take the derivative of \(H_n\)

\begin{equation}\label{eqn:hermiteDerivativeRecurranceRelation:50}
\begin{aligned}
(-1)^n D H_n
&= D \left( e^{x^2} D^n e^{-x^2} \right) \\
&=
2 x e^{x^2} D^n e^{-x^2}
+ e^{x^2} D^n \left( - 2 x e^{-x^2} \right) \\
&=
2 x e^{x^2} D^n e^{-x^2}
+ e^{x^2} \sum_{k=0}^n \binom{n}{k} D^k (-2 x) D^{n-k} e^{-x^2} \\
&=
2 x e^{x^2} D^n e^{-x^2}
+ e^{x^2} \sum_{k=0}^1 \binom{n}{k} D^k (-2 x) D^{n-k} e^{-x^2} \\
&=
\cancel{2 x e^{x^2} D^n e^{-x^2} }
+ e^{x^2} \left(
-\cancel{2 x D^{n} e^{-x^2} }
- 2 n D^{n-1} e^{-x^2}
\right)  \\
&=
- 2 n D^{n-1} e^{-x^2}
\end{aligned}
\end{equation}

So we have the rather simple end result

\begin{equation}\label{eqn:hermiteDerivativeRecurranceRelation:30}
\frac{d}{dx} H_n(x)
=
2 n H_{n-1}(x).
\end{equation}
