%
% Copyright Â© 2012 Peeter Joot.  All Rights Reserved.
% Licenced as described in the file LICENSE under the root directory of this GIT repository.
%

%\chapter{Relativistic motion in constant uniform electric or magnetic fields}
\label{chap:relativisticElectrodynamicsT3}
%\blogpage{http://sites.google.com/site/peeterjoot/math2011/relativisticElectrodynamicsT3.pdf}
%\date{Feb 3, 2011}

\makeproblem{Motion in an constant uniform Electric field}{pr:relativisticElectrodynamicsT3_1:1}{

Given
\begin{equation}\label{eqn:relativisticElectrodynamicsT3:}
\BE = E \xcap,
\end{equation}

We want to solve the problem
\begin{equation}\label{eqn:relativisticElectrodynamicsT3:20}
\BF = \frac{d\Bp}{dt} =
e \left( \BE + \frac{\Bv}{c} \cross \BB \right) = e \BE.
\end{equation}

Unlike second year classical physics, we will use relativistic momentum, so for only a constant electric field, our Lorentz force equation to solve becomes

\begin{equation}\label{eqn:relativisticElectrodynamicsT3:40}
\frac{d\Bp}{dt} = \frac{d (m \gamma \Bv)}{dt} = e \BE.
\end{equation}

} % makeproblem

\makeanswer{pr:relativisticElectrodynamicsT3_1:1}{

In components this is

\begin{equation}\label{eqn:relativisticElectrodynamicsT3:60}
\begin{aligned}
\pdot_x &= e E \\
\pdot_y &= \text{constant}
\end{aligned}
\end{equation}

Integrating the $x$ component we have
\begin{equation}\label{eqn:relativisticElectrodynamicsT3:65}
e E t + p_x(0)
=
\frac{m \xdot}{\sqrt{1 - (\xdot^2 + \ydot^2)/c^2}}
\end{equation}

If we let $p_x(0) = 0$, square and rearrange a bit we have

\begin{equation}\label{eqn:relativisticElectrodynamicsT3:70}
\frac{m^2}{(e E t)^2} \xdot^2 = 1 - \frac{\xdot^2 + \ydot^2}{c^2}
\end{equation}

For
\begin{equation}\label{eqn:relativisticElectrodynamicsT3:80}
\xdot^2 = \frac{c^2 - \ydot^2}{1 + (\frac{mc}{eEt})^2}.
\end{equation}

Now for the $y$ components, with $p_y(0) = p_0$, our equation to solve is

\begin{equation}\label{eqn:relativisticElectrodynamicsT3:82}
\frac{m \ydot}{\sqrt{1 - (\xdot^2 + \ydot^2)/c^2}} = p_0.
\end{equation}

Squaring this one we have
\begin{equation}\label{eqn:relativisticElectrodynamicsT3:84}
\frac{c^2 m^2}{p_0^2} \ydot^2 = c^2 - \xdot^2 - \ydot^2 ,
\end{equation}

and
\begin{equation}\label{eqn:relativisticElectrodynamicsT3:86}
\ydot^2 = \frac{ c^2 - \xdot^2}{1 + \frac{m^2 c^2}{p_0^2}}
\end{equation}

Observe that our energy is

\begin{equation}\label{eqn:relativisticElectrodynamicsT3:100}
\mathcal{E}^2 = p^2 c^2 + m^2 c^4,
\end{equation}

and for $t=0$
\begin{equation}\label{eqn:relativisticElectrodynamicsT3:100b}
\mathcal{E}_0^2 = p_0^2 c^2 + m^2 c^4.
\end{equation}

We can then write

\begin{equation}\label{eqn:relativisticElectrodynamicsT3:120}
\ydot^2 = \frac{ c^2 p_0^2 (c^2 - \xdot^2)}{ \mathcal{E}_0^2 }.
\end{equation}

Some messy substitution, using \eqnref{eqn:relativisticElectrodynamicsT3:80}, yields

\boxedEquation{eqn:relativisticElectrodynamicsT3:140}{
\begin{aligned}
\xdot &= \frac{c^2 e E t}{\sqrt{ \mathcal{E}_0^2 + (e c E t)^2 }} \\
\ydot &= \frac{c^2 p_0 }{\sqrt{ \mathcal{E}_0^2 + (e c E t)^2 }}
\end{aligned}
}


Solving for $x$ we have

\begin{equation}\label{eqn:relativisticElectrodynamicsT3:220}
x(t) = c^2 e E \int \frac{dt' t'}{\sqrt{ \mathcal{E}_0^2 + (e c E t')^2 }}
\end{equation}

Can solve with hyperbolic substitution or

\begin{equation}\label{eqn:relativisticElectrodynamicsT3:240}
x(t) = c^2 e E \int \frac{dt' t'}{\sqrt{ \mathcal{E}_0^2 + (e c E t')^2 }}
\end{equation}

\begin{equation}\label{eqn:relativisticElectrodynamicsT3:260}
d(u^2) = 2 u du \implies u du = \inv{2} d(u^2)
\end{equation}

\begin{equation}\label{eqn:relativisticElectrodynamicsT3:280}
x(t) = \frac{c^2 e E}{2 \mathcal{E}_0} \int \frac{d (u^2)}{\sqrt{ 1 + \left(\frac{e c E}{\mathcal{E}_0}\right)^2 u^2 }}
\end{equation}

Now we have something of the form

\begin{equation}\label{eqn:relativisticElectrodynamicsT3:290}
\int \frac{d v}{\sqrt{1 + a v}} = \frac{2}{a} \sqrt{1 + a v},
\end{equation}

so our final solution for $x(t)$ is

\begin{equation}\label{eqn:relativisticElectrodynamicsT3:300}
x(t) = \inv{e E} \sqrt{ \mathcal{E}_0^2 + (e c E t)^2 }
\end{equation}

or

\begin{equation}\label{eqn:relativisticElectrodynamicsT3:320}
x^2 - c^2 t^2 = \frac{\mathcal{E}_0^2}{ e^2 E^2 } = a^{-2}.
\end{equation}

Now for $y(t)$ we have

\begin{equation}\label{eqn:relativisticElectrodynamicsT3:340}
y(t) = c^2 p_0 \int \frac{dt}{ \sqrt{\mathcal{E}_0^2 + (e c E t)^2 }}
\end{equation}

\begin{equation}\label{eqn:relativisticElectrodynamicsT3:360}
t = \frac{\mathcal{E}_0}{ e c E} \sinh(u)
\end{equation}

\begin{equation}\label{eqn:relativisticElectrodynamicsT3:380}
dt = \frac{\mathcal{E}_0}{ e c E} \cosh(u) du
\end{equation}

\begin{equation}\label{eqn:relativisticElectrodynamicsT3:970}
\begin{aligned}
y(t) 
&= \frac{c^2 p_0}{\mathcal{E}_0} \int \frac{dt}{\sqrt{1 + (\frac{e c E}{\mathcal{E}_0})^2 t^2 }} \\
&= \frac{c^2 p_0}{\mathcal{E}_0} 
\frac{\mathcal{E}_0}{ e c E} 
\int \frac{ du \cosh u }{\sqrt{1 + \sinh^2 u }} \\
&= \frac{c p_0}{ e E} u 
\end{aligned}
\end{equation}

A final bit of substitution, including a sort of odd seeming parametrization of $x$ in terms of $y$ in terms of $t$, we have

\boxedEquation{eqn:relativisticElectrodynamicsT3:400}{
\begin{aligned}
y(t) &= \frac{c p_0}{ e E} \sinh^{-1} \left( \frac{e c E t}{\mathcal{E}_0} \right) \\
x(y) &= \frac{\mathcal{E}_0}{c E \cosh \left( \frac{y e E }{ c p_0} \right) }
\end{aligned}
}

\paragraph{Checks}

FIXME: check the checks.

\begin{equation}\label{eqn:relativisticElectrodynamicsT3:420}
v \rightarrow c, t \rightarrow \infty
\end{equation}

\begin{equation}\label{eqn:relativisticElectrodynamicsT3:440}
v << c, t \rightarrow 0
\end{equation}

\begin{equation}\label{eqn:relativisticElectrodynamicsT3:990}
\begin{aligned}
m v_x &= e E t + ... \\
x &\sim t^2 
\end{aligned}
\end{equation}

\begin{equation}\label{eqn:relativisticElectrodynamicsT3:460}
m v_y = p_0 \rightarrow y \sim t
\end{equation}

\begin{equation}\label{eqn:relativisticElectrodynamicsT3:480}
x(y) \sim y^2
\end{equation}

(a parabola)

\paragraph{An alternate way}

There is also a tricky way (as in the text), with 

\begin{equation}\label{eqn:relativisticElectrodynamicsT3:160}
\begin{aligned}
\Bp &= m \gamma \Bv  \\
\mathcal{E} &= \gamma m c^2 
\end{aligned}
\end{equation}

We can solve this for $\Bp$

\begin{equation}\label{eqn:relativisticElectrodynamicsT3:1010}
\begin{aligned}
m \gamma &= \frac{\Bp \cdot \Bv}{\Bv^2} = \frac{\mathcal{E}}{c^2} \\
\Bp \cross \Bv &= 0
\end{aligned}
\end{equation}

With the cross product zero, $\Bp$ has only a component in the direction of $\Bv$, and we can invert to yield

\begin{equation}\label{eqn:relativisticElectrodynamicsT3:180}
\Bp = \frac{\mathcal{E} \Bv}{c^2}.
\end{equation}

This implies

\begin{equation}\label{eqn:relativisticElectrodynamicsT3:200}
\xdot = \frac{c^2 p_x}{\mathcal{E}},
\end{equation}

and one can work from there as well.

} % makeanswer
