%
% Copyright © 2016 Peeter Joot.  All Rights Reserved.
% Licenced as described in the file LICENSE under the root directory of this GIT repository.
%
\makeproblem{Poynting theorem}{emt:problemSet7:1}{
Using Maxwell's equations given in the class notes, derive the Poynting theorem in both
differential and integral form for instantaneous fields. Assume a linear, homogeneous medium
with no temporal dispersion.
} % makeproblem

\makeanswer{emt:problemSet7:1}{

Given
\begin{equation}\label{eqn:emtproblemSet7Problem1:20}
\spacegrad \cross \BE
= -\BM_i - \PD{t}{\BB},
\end{equation}

and
\begin{equation}\label{eqn:emtproblemSet7Problem1:40}
\spacegrad \cross \BH
= \BJ_i + \BJ_c + \PD{t}{\BD},
\end{equation}

we want to expand the divergence of \( \BE \cross \BH \) to find the form of the Poynting theorem.


First we need the chain rule for of this sort of divergence.  Using primes to indicate the scope of the gradient operation

\begin{dmath}\label{eqn:emtproblemSet7Problem1:60}
\spacegrad \cdot \lr{ \BE \cross \BH }
=
\spacegrad' \cdot \lr{ \BE' \cross \BH }
-
\spacegrad' \cdot \lr{ \BH' \cross \BE }
=
\BH \cdot \lr{ \spacegrad' \cross \BE' }
-
\BH \cdot \lr{ \spacegrad' \cross \BH' }
%= %\gpgradezero{ %\spacegrad \lr{ \BE \cross \BH }
%}
%=
%\gpgradezero{
%-I \spacegrad \lr{ \BE \wedge \BH }
%}
%=
%-I \spacegrad \wedge \lr{ \BE \wedge \BH }
%=
%-I \BH \wedge \lr{ \spacegrad \wedge \BE }
%+I \BE \wedge \lr{ \spacegrad \wedge \BH }
=
\BH \cdot \lr{ \spacegrad \cross \BE }
-
\BE \cdot \lr{ \spacegrad \cross \BH }.
\end{dmath}

In the second step, cyclic permutation of the triple product was used.
This checks against the inside front cover of Jackson \citep{jackson1975cew}.  Now we can plug in the Maxwell equation cross products.

\begin{dmath}\label{eqn:emtproblemSet7Problem1:80}
\spacegrad \cdot \lr{ \BE \cross \BH }
=
\BH \cdot \lr{ -\BM_i - \PD{t}{\BB} }
-
\BE \cdot \lr{ \BJ_i + \BJ_c + \PD{t}{\BD} }
=
-\BH \cdot \BM_i
-\mu \BH \cdot \PD{t}{\BH}
-
\BE \cdot \BJ_i
-
\BE \cdot \BJ_c
-
\epsilon \BE \cdot \PD{t}{\BE},
\end{dmath}

or

%\begin{dmath}\label{eqn:emtproblemSet7Problem1:100}
\boxedEquation{eqn:emtproblemSet7Problem1:120}{
0
=
\spacegrad \cdot \lr{ \BE \cross \BH }
+ \frac{\epsilon}{2} \PD{t}{} \Abs{ \BE }^2
+ \frac{\mu}{2} \PD{t}{} \Abs{ \BH }^2
+ \BH \cdot \BM_i
+ \BE \cdot \BJ_i
+ \sigma \Abs{\BE}^2.
}
%\end{dmath}

In integral form this is

\begin{dmath}\label{eqn:emtproblemSet7Problem1:140}
0
=
\int d\BA \cdot \lr{ \BE \cross \BH }
+ \inv{2} \PD{t}{} \int dV \lr{
\epsilon \Abs{ \BE }^2
+ \mu \Abs{ \BH }^2
}
+ \int dV \BH \cdot \BM_i
+ \int dV \BE \cdot \BJ_i
+ \sigma \int dV \Abs{\BE}^2.
\end{dmath}

}
